more on examples

theories/crypto/PKE.ec
@@ -7,6 +7,8 @@
  * -------------------------------------------------------------------- *)
 
 require import AllCore List Distr DBool LorR.
+require (*--*) CHoareTactic.
+(*---*) import StdBigop.Bigint BIA.
 
 type pkey.
 type skey.
@@ -17,6 +19,20 @@ module type Scheme = {
   proc kg() : pkey * skey
   proc enc(pk:pkey, m:plaintext)  : ciphertext
   proc dec(sk:skey, c:ciphertext) : plaintext option
+}.
+
+module Correctness (S:Scheme) = {
+  proc main(m:plaintext) : bool = {
+    var pk : pkey;
+    var sk : skey;
+    var c  : ciphertext;
+    var m' : plaintext option;
+
+    (pk, sk) <@ S.kg();
+    c        <@ S.enc(pk, m);
+    m'       <@ S.dec(sk, c);
+    return (m' = Some m);
+  }
 }.
 
 module type Adversary = {
@@ -103,9 +119,6 @@ end section.
 ** Also, oracle annotations could be used to provide different oracles during
 ** the choose and guess stages of the experiment.
 *)
-const qD : int.
-
-axiom qD_pos : 0 < qD.
 
 module type CCA_ORC = {
   proc dec(c:ciphertext) : plaintext option
@@ -117,17 +130,48 @@ module type CCA_ADV (O:CCA_ORC) = {
 }.
 
 module CCA (S:Scheme, A:CCA_ADV) = {
-  var log : ciphertext list
+  var log   : ciphertext list
   var cstar : ciphertext option
-  var sk : skey
+  var sk    : skey
 
   module O = {
     proc dec(c:ciphertext) : plaintext option = {
       var m : plaintext option;
 
-      if (size log < qD && (Some c <> cstar)) {
-        log <- c :: log;
-        m   <@ S.dec(sk, c);
+      if (Some c <> cstar) m <@ S.dec(sk, c);
+      else m <- None;
+      return m;
+    }
+  }
+
+  module A = A(O)
+
+  proc main() : bool = {
+    var pk : pkey;
+    var m0, m1 : plaintext;
+    var c : ciphertext;
+    var b, b' : bool;
+
+    cstar    <- None;
+    (pk, sk) <@ S.kg();
+    (m0, m1) <@ A.choose(pk);
+    b        <$ {0,1};
+    c        <@ S.enc(pk, b ? m1 : m0);
+    cstar    <- Some c;
+    b'       <@ A.guess(c);
+    return (b' = b);
+  }
+}.
+
+module CCAl (S:Scheme, A:CCA_ADV) = {
+
+  module O = {
+    proc dec(c:ciphertext) : plaintext option = {
+      var m : plaintext option;
+
+      if (Some c <> CCA.cstar) {
+        CCA.log <- c :: CCA.log;
+        m   <@ S.dec(CCA.sk, c);
       }
       else m <- None;
       return m;
@@ -142,28 +186,191 @@ module CCA (S:Scheme, A:CCA_ADV) = {
     var c : ciphertext;
     var b, b' : bool;
 
-    log      <- [];
-    cstar    <- None;
-    (pk, sk) <@ S.kg();
+    CCA.log      <- [];
+    CCA.cstar    <- None;
+    (pk, CCA.sk) <@ S.kg();
     (m0, m1) <@ A.choose(pk);
     b        <$ {0,1};
     c        <@ S.enc(pk, b ? m1 : m0);
-    cstar    <- Some c;
+    CCA.cstar    <- Some c;
     b'       <@ A.guess(c);
     return (b' = b);
   }
 }.
 
-module Correctness (S:Scheme) = {
-  proc main(m:plaintext) : bool = {
-    var pk : pkey;
-    var sk : skey;
-    var c  : ciphertext;
-    var m' : plaintext option;
+section.
 
-    (pk, sk) <@ S.kg();
-    c        <@ S.enc(pk, m);
-    m'       <@ S.dec(sk, c);
-    return (m' = Some m);
+declare module S: Scheme {-CCA}.
+
+declare module A: CCA_ADV {-CCA, -S}.
+
+equiv eq_CCA_CCAl : CCA(S,A).main ~ CCAl(S,A).main : ={glob S, glob A} ==> ={res, glob S, glob A, CCA.sk, CCA.cstar}.
+proof. by sim. qed.
+
+end section.
+
+(* Complexity of the adversary *)
+type cost_A = {
+  cchoose   : int;
+  qD_choose : int;
+  cguess    : int;
+  qD_guess  : int;
+}.
+
+type cost_S = {
+  ckg  : int;
+  cenc : int;
+  cdec : int;
+}.
+
+abstract theory CCA_q.
+
+op cA : cost_A.
+
+axiom ge0_cA : 0 <= cA.`cchoose /\ 0 <= cA.`qD_choose /\ 0 <= cA.`cguess /\ 0 <= cA.`qD_guess.
+
+op qD = cA.`qD_choose + cA.`qD_guess.
+
+lemma ge0_qD : 0 <= qD by smt (ge0_cA).
+
+op cS : cost_S.
+
+axiom ge0_cS : 0 <= cS.`ckg /\ 0 <= cS.`cenc /\ 0 <= cS.`cdec.
+
+op ceqocipher : int.
+
+schema cost_eqcipher `{P} {c1 c2 : ciphertext option} : cost [P : c1 = c2] = cost[P:c1] + cost[P:c2] + ceqocipher .
+hint simplify cost_eqcipher.
+
+module CCAq (S:Scheme, A:CCA_ADV) = {
+ 
+  module O = {
+    proc dec(c:ciphertext) : plaintext option = {
+      var m : plaintext option;
+
+      if (size CCA.log < qD && (Some c <> CCA.cstar)) {
+        CCA.log <- c :: CCA.log;
+        m   <@ S.dec(CCA.sk, c);
+      }
+      else m <- None;
+      return m;
+    }
+  }
+
+  module A = A(O)
+
+  proc main() : bool = {
+    var pk : pkey;
+    var m0, m1 : plaintext;
+    var c : ciphertext;
+    var b, b' : bool;
+
+    CCA.log      <- [];
+    CCA.cstar    <- None;
+    (pk, CCA.sk) <@ S.kg();
+    (m0, m1) <@ A.choose(pk);
+    b        <$ {0,1};
+    c        <@ S.enc(pk, b ? m1 : m0);
+    CCA.cstar    <- Some c;
+    b'       <@ A.guess(c);
+    return (b' = b);
   }
 }.
+
+section.
+
+declare module S: Scheme [kg  : `{cS.`ckg},
+                          enc : `{cS.`cenc}, 
+                          dec : `{cS.`cdec} ]
+                         {-CCA}.
+
+lemma Sdec_ll : islossless S.dec.
+proof.
+have h : choare [S.dec : true ==> true] time [cS.`cdec].
++ by proc true : time [].
+conseq h.
+qed.
+
+lemma Senc_ll : islossless S.enc.
+proof.
+have h : choare [S.enc : true ==> true] time [cS.`cenc].
++ by proc true : time [].
+conseq h.
+qed.
+
+declare module A : CCA_ADV [choose : `{cA.`cchoose, #O.dec : cA.`qD_choose},
+                            guess  : `{cA.`cguess, #O.dec : cA.`qD_guess}]
+                           {-CCA, -S}.
+
+axiom Achoose_ll : forall (O <: CCA_ORC {-A}), islossless O.dec => islossless A(O).choose.
+axiom Aguess_ll : forall (O <: CCA_ORC {-A}), islossless O.dec => islossless A(O).guess.
+
+lemma CCAl_cbound : choare [CCAl(S,A).main : true ==> size CCA.log <= qD] time 
+                          [ 5 + cdbool + (3 + ceqocipher) * cA.`qD_guess +  (3 + ceqocipher) * cA.`qD_choose;
+                            S.kg  : 1; S.enc : 1; S.dec : qD;
+                            A.choose : 1; A.guess  : 1].
+proof.
+  proc.
+  call (:true; 
+         (CCAl(S,A).O.dec : size CCA.log - cA.`qD_choose) 
+           time
+           [(CCAl(S,A).O.dec : [fun _ => 3 + ceqocipher; S.dec: fun _ => 1])]).
+  + move=> zdec hzdec; proc.
+    if. 
+    + by call (:true; time []); auto => &hr /> * /#.
+    by auto => &hr />; smt(ge0_cS).
+  wp; call (:true; time []); rnd.
+  call (:true; 
+         (CCAl(S,A).O.dec : size CCA.log) 
+           time
+           [(CCAl(S,A).O.dec : [fun _ => 3 + ceqocipher; S.dec: fun _ => 1])]).
+  + move=> zdec hzdec; proc.
+    if. 
+    + by call (:true; time []); auto => &hr /> * /#.
+    by auto => &hr />; smt(ge0_cS).
+  call(:true; time[]); auto => />. rewrite dbool_ll /=; split. smt().
+  by rewrite !bigi_constz; smt(ge0_cA).
+qed.
+
+lemma CCAl_bound : hoare [CCAl(S,A).main : true ==> size CCA.log <= qD].
+proof. conseq CCAl_cbound. qed.
+
+equiv CCAq_CCAl : CCAq(S,A).main ~ CCAl(S,A).main : ={glob A, glob S} ==> ={res, glob S, glob A, glob CCA}.
+proof.
+  conseq (_: ={glob A, glob S} ==> size CCA.log{2} <= qD => ={res, glob S, glob A, glob CCA}) 
+    _ (CCAl_bound) => //.
+  proc.  
+  seq 5 5 : (={b} /\ (size CCA.log{2} <= qD => ={pk, m0, m1, glob S, glob A, glob CCA})).
+  rnd; call (: qD < size CCA.log, ={glob S, glob CCA}) => //=.
+  + by apply Achoose_ll.  
+  + proc; if{2}; last by rcondf{1} ^if; auto.
+    if{1}; 1: by call (:true); auto.
+    by call{2} Sdec_ll; auto => /> /#.
+  + by move=> _ _; islossless; apply Sdec_ll.
+  + proc; if; auto.
+    by call Sdec_ll; auto => /#.
+  call (:true); auto => />; smt().
+
+  call (: qD < size CCA.log, ={glob S, glob CCA}) => //=.
+  + by apply Aguess_ll.  
+  + proc; if{2}; last by rcondf{1} ^if; auto.
+    if{1}; 1: by call (:true); auto.
+    by call{2} Sdec_ll; auto => /> /#.
+  + by move=> _ _; islossless; apply Sdec_ll.
+  + proc; if; auto.
+    by call Sdec_ll; auto => /#.
+  
+  wp; case: (size CCA.log{2} <= qD).
+  + by call (:true); auto => /> /#.
+  by call{1} Senc_ll; call{2} Senc_ll; skip => /> /#.
+qed.
+
+equiv CCA_CCAq : CCA(S,A).main ~ CCAq(S,A).main : ={glob A, glob S} ==> ={res, glob S, glob A, CCA.sk, CCA.cstar}.
+proof.
+  transitivity CCAl(S,A).main
+     (={glob A, glob S} ==> ={res, glob S, glob A, CCA.sk, CCA.cstar})
+     (={glob A, glob S} ==> ={res, glob S, glob A, glob CCA})=> //; 1: smt().
+  + by sim.
+  by symmetry; conseq CCAq_CCAl.
+qed.
+
